cogent/examples/wa_connect/WordArray_CorresProof_Asm.thy
@@ -61,47 +61,63 @@ lemma val_proc_env_matches_\<xi>m_\<Xi>:
    apply (rule_tac x = x in exI; simp)
   done
 
-lemma proc_env_u_v_matches_\<xi>0_\<xi>m_\<Xi>:
-  "proc_env_u_v_matches \<xi>0 \<xi>m \<Xi>"
-  apply (clarsimp simp: proc_env_u_v_matches_def)
-  apply (subst (asm) \<Xi>_def)
-  apply (subst (asm) assoc_lookup.simps)+
-  apply (clarsimp split: if_split_asm)
-    apply (clarsimp simp: upd_wa_get_0_def wordarray_get_0_type_def abbreviatedType6_def)
-    apply (erule u_v_recE'; clarsimp)
-    apply (erule u_v_r_consE'; clarsimp)
-    apply (erule u_v_p_absE'; clarsimp)
-    apply (erule u_v_r_consE'; clarsimp)
-    apply (erule u_v_r_emptyE')
-    apply (erule u_v_primE')+
-    apply (subst (asm) lit_type.simps)+
-    apply clarsimp
-    apply (rule conjI)
-     apply (clarsimp simp: val_wa_get_0_def)
-     apply (rule_tac x = "{}" in exI)+
-     apply (clarsimp simp: abs_upd_val'_def frame_def word_less_nat_alt)
-     apply (erule_tac x = idx in allE)
-     apply clarsimp
-     apply (case_tac "unat idx < length xs"; clarsimp intro!: u_v_prim[where l = "(LU32 _)", simplified])
-    apply (clarsimp simp: word_less_nat_alt abs_upd_val'_def)
-    apply (case_tac a'; clarsimp simp: word_less_nat_alt)
-    apply (erule_tac x = idx in allE)
-    apply (case_tac "unat idx < length x1"; clarsimp)
-     apply (rule_tac x = "VPrim (LU32 x)" in exI)
-     apply (clarsimp simp: val_wa_get_0_def)
-    apply (rule_tac x = "VPrim (LU32 0)" in exI)
-    apply (clarsimp simp: val_wa_get_0_def)
-   apply (clarsimp simp: upd_wa_length_0_def wordarray_length_0_type_def)
-   apply (erule u_v_p_absE'; clarsimp)
-   apply (clarsimp simp: abs_upd_val'_def)
-   apply (case_tac a'a; clarsimp)
-   apply (rule conjI)
-    apply (clarsimp simp: val_wa_length_0_def)
-    apply (rule_tac x = "{}" in exI)+
-    apply (clarsimp simp: frame_def intro!: u_v_prim[where l = "(LU32 _)", simplified])
-   apply (clarsimp simp: abs_upd_val'_def)
-   apply (rule_tac x = "VPrim (LU32 len)" in exI)
+lemma wordarray_get_upd_val:
+  "\<And>K a b \<sigma> \<sigma>' \<tau>s aa a' v v' r w.
+   \<lbrakk>list_all2 (kinding []) \<tau>s K; wordarray_get_0_type = (K, a, b);
+    upd_val_rel \<Xi> \<sigma> aa a' (instantiate \<tau>s a) r w; upd_wa_get_0 (\<sigma>, aa) (\<sigma>', v)\<rbrakk>
+    \<Longrightarrow> (val_wa_get_0 a' v' \<longrightarrow> (\<exists>r' w'. upd_val_rel \<Xi> \<sigma>' v v' (instantiate \<tau>s b) r' w' \<and> r' \<subseteq> r \<and> 
+          frame \<sigma> w \<sigma>' w')) \<and> Ex (val_wa_get_0 a')"
+  apply (clarsimp simp: upd_wa_get_0_def wordarray_get_0_type_def abbreviatedType6_def)
+  apply (erule u_v_recE'; clarsimp)
+  apply (erule u_v_r_consE'; clarsimp)
+  apply (erule u_v_p_absE'; clarsimp)
+  apply (erule u_v_r_consE'; clarsimp)
+  apply (erule u_v_r_emptyE')
+  apply (erule u_v_primE')+
+  apply (subst (asm) lit_type.simps)+
+  apply clarsimp
+  apply (rule conjI)
+   apply (clarsimp simp: val_wa_get_0_def)
+   apply (rule_tac x = "{}" in exI)+
+   apply (clarsimp simp: abs_upd_val'_def frame_def word_less_nat_alt)
+   apply (erule_tac x = idx in allE)
+   apply clarsimp
+   apply (case_tac "unat idx < length xs"; clarsimp intro!: u_v_prim[where l = "(LU32 _)", simplified])
+  apply (clarsimp simp: word_less_nat_alt abs_upd_val'_def)
+  apply (case_tac a'; clarsimp simp: word_less_nat_alt)
+  apply (erule_tac x = idx in allE)
+  apply (case_tac "unat idx < length x1"; clarsimp)
+   apply (rule_tac x = "VPrim (LU32 x)" in exI)
+   apply (clarsimp simp: val_wa_get_0_def)
+  apply (rule_tac x = "VPrim (LU32 0)" in exI)
+  apply (clarsimp simp: val_wa_get_0_def)
+  done
+
+lemma wordarray_length_upd_val:
+  "\<And>K a b \<sigma> \<sigma>' \<tau>s aa a' v v' r w.
+   \<lbrakk>list_all2 (kinding []) \<tau>s K; wordarray_length_0_type = (K, a, b);
+    upd_val_rel \<Xi> \<sigma> aa a' (instantiate \<tau>s a) r w; upd_wa_length_0 (\<sigma>, aa) (\<sigma>', v)\<rbrakk>
+    \<Longrightarrow> (val_wa_length_0 a' v' \<longrightarrow> (\<exists>r' w'. upd_val_rel \<Xi> \<sigma>' v v' (instantiate \<tau>s b) r' w' \<and> r' \<subseteq> r \<and> 
+          frame \<sigma> w \<sigma>' w')) \<and> Ex (val_wa_length_0 a')"
+  apply (clarsimp simp: upd_wa_length_0_def wordarray_length_0_type_def)
+  apply (erule u_v_p_absE'; clarsimp)
+  apply (clarsimp simp: abs_upd_val'_def)
+  apply (case_tac a'a; clarsimp)
+  apply (rule conjI)
    apply (clarsimp simp: val_wa_length_0_def)
+   apply (rule_tac x = "{}" in exI)+
+   apply (clarsimp simp: frame_def intro!: u_v_prim[where l = "(LU32 _)", simplified])
+  apply (clarsimp simp: abs_upd_val'_def)
+  apply (rule_tac x = "VPrim (LU32 len)" in exI)
+  apply (clarsimp simp: val_wa_length_0_def)
+  done
+
+lemma wordarray_put2_upd_val:
+  "\<And>K a b \<sigma> \<sigma>' \<tau>s aa a' v v' r w.
+   \<lbrakk>list_all2 (kinding []) \<tau>s K; wordarray_put2_0_type = (K, a, b); 
+    upd_val_rel \<Xi> \<sigma> aa a' (instantiate \<tau>s a) r w; upd_wa_put2_0 (\<sigma>, aa) (\<sigma>', v)\<rbrakk>
+    \<Longrightarrow> (val_wa_put2_0 a' v' \<longrightarrow> (\<exists>r' w'. upd_val_rel \<Xi> \<sigma>' v v' (instantiate \<tau>s b) r' w' \<and> r' \<subseteq> r \<and>
+          frame \<sigma> w \<sigma>' w')) \<and> Ex (val_wa_put2_0 a')"
   apply (clarsimp simp: upd_wa_put2_0_def wordarray_put2_0_type_def abbreviatedType5_def)
   apply (erule u_v_recE'; clarsimp)
   apply (erule u_v_r_consE'; clarsimp)
@@ -150,12 +166,12 @@ lemma proc_env_u_v_matches_\<xi>0_\<xi>m_\<Xi>:
      apply (erule_tac x = idx in allE)
      apply clarsimp
     apply simp
-   apply (clarsimp simp: frame_def)
+   apply (clarsimp simp: frame_def abs_upd_val'_def abs_typing_u_def)
+  apply (case_tac a; clarsimp)
    apply (rule conjI; clarsimp)
     apply (rule conjI)
-     apply (clarsimp simp: abs_upd_val'_def abs_typing_u_def)
+     apply clarsimp
     apply (rule conjI; clarsimp)
-    apply (clarsimp simp: abs_upd_val'_def abs_typing_u_def)
    apply (rule conjI; clarsimp)
   apply (clarsimp simp: abs_upd_val'_def)
   apply (case_tac a; clarsimp simp: abs_typing_u_def)
@@ -164,28 +180,51 @@ lemma proc_env_u_v_matches_\<xi>0_\<xi>m_\<Xi>:
   apply (clarsimp simp: val_wa_put2_0_def)
   done
 
-lemma upd_proc_env_matches_ptrs_\<xi>0_\<Xi>:
-  "upd.proc_env_matches_ptrs \<xi>0 \<Xi>"
-  apply (unfold upd.proc_env_matches_ptrs_def)
-  apply clarsimp
+lemma proc_env_u_v_matches_\<xi>0_\<xi>m_\<Xi>:
+  "proc_env_u_v_matches \<xi>0 \<xi>m \<Xi>"
+  apply (clarsimp simp: proc_env_u_v_matches_def)
   apply (subst (asm) \<Xi>_def)
   apply (subst (asm) assoc_lookup.simps)+
   apply (clarsimp split: if_split_asm)
-    apply (clarsimp simp: wordarray_get_0_type_def abbreviatedType6_def upd_wa_get_0_def)
-    apply (erule upd.u_t_recE; clarsimp)
-    apply (erule upd.u_t_r_consE; clarsimp)
-    apply (erule upd.u_t_p_absE; clarsimp)
-    apply (erule upd.u_t_r_consE; clarsimp)
-    apply (erule upd.u_t_r_emptyE; clarsimp)
-    apply (erule upd.u_t_primE; subst (asm) lit_type.simps; clarsimp)+
-    apply (rule_tac x = "{}" in exI)+
-    apply (clarsimp simp: frame_def abs_typing_u_def)
-    apply (erule_tac x = idx in allE)
-    apply (case_tac "idx < len"; clarsimp intro!: upd.u_t_prim[where l = "(LU32 _)", simplified])
-   apply (clarsimp simp: wordarray_length_0_type_def upd_wa_length_0_def)
-   apply (erule upd.u_t_p_absE; clarsimp)
-   apply (rule_tac x = "{}" in exI)+
-   apply (clarsimp simp: frame_def intro!: upd.u_t_prim[where l = "(LU32 _)", simplified])
+    apply (clarsimp simp: wordarray_get_upd_val)
+   apply (clarsimp simp: wordarray_length_upd_val)
+  apply (clarsimp simp: wordarray_put2_upd_val)
+  done
+
+lemma wordarray_get_uval_typing_frame:
+  "\<And>K a b \<sigma> \<sigma>' \<tau>s v v' r w.
+   \<lbrakk>list_all2 (kinding []) \<tau>s K; wordarray_get_0_type = (K, a, b);
+    upd.uval_typing \<Xi> \<sigma> v (instantiate \<tau>s a) r w; upd_wa_get_0 (\<sigma>, v) (\<sigma>', v')\<rbrakk>
+    \<Longrightarrow> \<exists>r' w'. upd.uval_typing \<Xi> \<sigma>' v' (instantiate \<tau>s b) r' w' \<and> r' \<subseteq> r \<and> frame \<sigma> w \<sigma>' w'"
+  apply (clarsimp simp: wordarray_get_0_type_def abbreviatedType6_def upd_wa_get_0_def)
+  apply (erule upd.u_t_recE; clarsimp)
+  apply (erule upd.u_t_r_consE; clarsimp)
+  apply (erule upd.u_t_p_absE; clarsimp)
+  apply (erule upd.u_t_r_consE; clarsimp)
+  apply (erule upd.u_t_r_emptyE; clarsimp)
+  apply (erule upd.u_t_primE; subst (asm) lit_type.simps; clarsimp)+
+  apply (rule_tac x = "{}" in exI)+
+  apply (clarsimp simp: frame_def abs_typing_u_def)
+  apply (erule_tac x = idx in allE)
+  apply (case_tac "idx < len"; clarsimp intro!: upd.u_t_prim[where l = "(LU32 _)", simplified])
+  done
+
+lemma wordarray_length_uval_typing_frame:
+  "\<And>K a b \<sigma> \<sigma>' \<tau>s v v' r w.
+   \<lbrakk>list_all2 (kinding []) \<tau>s K; wordarray_length_0_type = (K, a, b); 
+    upd.uval_typing \<Xi> \<sigma> v (instantiate \<tau>s a) r w; upd_wa_length_0 (\<sigma>, v) (\<sigma>', v')\<rbrakk>
+    \<Longrightarrow> \<exists>r' w'. upd.uval_typing \<Xi> \<sigma>' v' (instantiate \<tau>s b) r' w' \<and> r' \<subseteq> r \<and> frame \<sigma> w \<sigma>' w'"
+  apply (clarsimp simp: wordarray_length_0_type_def upd_wa_length_0_def)
+  apply (erule upd.u_t_p_absE; clarsimp)
+  apply (rule_tac x = "{}" in exI)+
+  apply (clarsimp simp: frame_def intro!: upd.u_t_prim[where l = "(LU32 _)", simplified])
+  done
+
+lemma wordarray_put2_uval_typing_frame:
+  "\<And>K a b \<sigma> \<sigma>' \<tau>s v v' r w.
+   \<lbrakk>list_all2 (kinding []) \<tau>s K; wordarray_put2_0_type = (K, a, b);
+    upd.uval_typing \<Xi> \<sigma> v (instantiate \<tau>s a) r w; upd_wa_put2_0 (\<sigma>, v) (\<sigma>', v')\<rbrakk>
+    \<Longrightarrow> \<exists>r' w'. upd.uval_typing \<Xi> \<sigma>' v' (instantiate \<tau>s b) r' w' \<and> r' \<subseteq> r \<and> frame \<sigma> w \<sigma>' w'"
   apply (clarsimp simp: wordarray_put2_0_type_def abbreviatedType5_def upd_wa_put2_0_def)
   apply (erule upd.u_t_recE; clarsimp)
   apply (erule upd.u_t_r_consE; clarsimp)
@@ -215,12 +254,22 @@ lemma upd_proc_env_matches_ptrs_\<xi>0_\<Xi>:
    apply (clarsimp simp: frame_def abs_typing_u_def)
    apply (rule conjI; clarsimp)
     apply (rule conjI)
-     apply (rule disjI2)
-     apply (rule disjI2)
-     apply (rule_tac x = idx in exI; simp)
+     apply clarsimp
     apply (rule conjI; clarsimp)
    apply (rule conjI; clarsimp)
   apply (clarsimp simp: abs_typing_u_def)
+  done
+
+lemma upd_proc_env_matches_ptrs_\<xi>0_\<Xi>:
+  "upd.proc_env_matches_ptrs \<xi>0 \<Xi>"
+  apply (unfold upd.proc_env_matches_ptrs_def)
+  apply clarsimp
+  apply (subst (asm) \<Xi>_def)
+  apply (subst (asm) assoc_lookup.simps)+
+  apply (clarsimp split: if_split_asm)
+    apply (clarsimp simp: wordarray_get_uval_typing_frame)
+   apply (clarsimp simp: wordarray_length_uval_typing_frame)
+  apply (clarsimp simp: wordarray_put2_uval_typing_frame)
   done
 
 lemma proc_ctx_wellformed_\<Xi>:
@@ -239,6 +288,542 @@ lemma proc_ctx_wellformed_\<Xi>:
                         mul_type_def mul_arr_type_def)
   done
 
+
+lemma wordarray_fold_no_break_uval_typing_frame:
+  "\<And>K a b \<sigma> \<sigma>' \<tau>s v v' r w.
+   \<lbrakk>list_all2 (kinding []) \<tau>s K; wordarray_fold_no_break_0_type = (K, a, b);
+    upd.uval_typing \<Xi> \<sigma> v (instantiate \<tau>s a) r w; upd_wa_foldnb_0 (\<sigma>, v) (\<sigma>', v')\<rbrakk>
+    \<Longrightarrow> \<exists>r' w'. upd.uval_typing \<Xi> \<sigma>' v' (instantiate \<tau>s b) r' w' \<and> r' \<subseteq> r \<and> frame \<sigma> w \<sigma>' w'"
+  apply (clarsimp simp: wordarray_fold_no_break_0_type_def upd_wa_foldnb_0_def)
+  apply (rule_tac x = "{}" in exI)
+  apply (rule_tac x = w in exI)
+  apply (clarsimp simp: frame_def)
+  apply (erule upd.u_t_recE; clarsimp)
+  apply (case_tac fs; clarsimp)
+  apply (case_tac list; clarsimp)
+  apply (case_tac lista; clarsimp)
+  apply (case_tac list; clarsimp)
+  apply (case_tac lista; clarsimp)
+  apply (case_tac list; clarsimp)
+  apply (erule upd.u_t_r_consE; clarsimp)
+  apply (erule upd.u_t_p_absE; clarsimp)
+  apply (erule upd.u_t_r_consE; simp)
+  apply (erule conjE)+
+  apply (subst (asm) type_repr.simps[symmetric])+
+  apply clarsimp
+  apply (erule upd.u_t_r_consE; simp)
+  apply (erule conjE)+
+  apply (subst (asm) type_repr.simps[symmetric])+
+  apply clarsimp
+  apply (erule upd.u_t_r_consE; simp)
+  apply (erule conjE)+
+  apply (subst (asm) type_repr.simps[symmetric])+
+  apply clarsimp
+  apply (erule upd.u_t_r_consE; simp)
+  apply (erule conjE)+
+  apply (subst (asm) type_repr.simps[symmetric])+
+  apply clarsimp
+  apply (erule upd.u_t_r_consE; simp)
+  apply (erule conjE)+
+  apply clarsimp
+  apply (erule upd.u_t_r_emptyE)
+  apply (erule upd.u_t_primE)+
+  apply (subst (asm) lit_type.simps)+
+  apply clarsimp
+  apply (erule upd.u_t_unitE)
+  apply clarsimp
+  apply (case_tac xa; clarsimp)
+   apply (erule upd.u_t_funE'; clarsimp)
+   apply (rule upd.u_t_prim[where l = "LU32 _", simplified])
+  apply (erule upd.u_t_afunE; clarsimp)
+  apply (rule upd.u_t_prim[where l = "LU32 _", simplified])
+  done
+
+inductive_cases v_t_prim_tE : "val.vval_typing \<Xi>' v (TPrim (Num U32))"
+
+lemma lit_type_ex_32:
+  "lit_type l = Num U32 \<Longrightarrow> \<exists>v. l = LU32 v"
+  apply (induct l; clarsimp)
+  done
+
+lemma val_wa_foldnb_0_mono_helper1:
+  "\<lbrakk>val.proc_env_matches \<xi>m1 \<Xi>; proc_ctx_wellformed \<Xi>; \<forall>i<length xs. \<exists>v. xs ! i = VPrim (LU32 v);
+    \<Xi>, [], [option.Some Generated_TypeProof.abbreviatedType1] \<turnstile> App (Fun (val.rename_expr rename 
+      (val.monoexpr (specialise ts f))) []) (Var 0) : TPrim (Num U32);
+    val_wa_foldnb_bod_0 xs frm to (Fun (val.rename_expr rename (val.monoexpr (specialise ts f))) [])
+         (VPrim (LU32 acc)) VUnit (VPrim (LU32 r))\<rbrakk>
+       \<Longrightarrow> val_wa_foldnb_bod_0p xs frm to (Fun f ts) (VPrim (LU32 acc)) VUnit (VPrim (LU32 r))"
+  apply (induct to arbitrary: r)
+   apply (erule val_wa_foldnb_bod_0.elims; clarsimp)
+   apply (subst val_wa_foldnb_bod_0p.simps; clarsimp)
+  apply clarsimp
+  apply (case_tac "length xs < Suc to")
+   apply (erule_tac x = r in meta_allE)
+   apply (drule val_wa_foldnb_bod_0_back_step'; simp)
+   apply (drule val_wa_foldnb_bod_0p_to_geq_lenD)
+    apply linarith
+   apply (rule val_wa_foldnb_bod_0p_to_geq_len; simp)
+  apply (clarsimp simp: not_less)
+  apply (case_tac "frm \<ge> to")
+   apply (erule val_wa_foldnb_bod_0.elims; clarsimp split: if_splits)
+    apply (erule val_wa_foldnb_bod_0.elims; clarsimp)
+    apply (subst val_wa_foldnb_bod_0p.simps; clarsimp)
+    apply (subst val_wa_foldnb_bod_0p.simps; clarsimp)
+    apply (drule_tac \<gamma> = "[VRecord [VPrim (LU32 v), VPrim (LU32 acc), VUnit]]" and
+      \<Gamma> = "[option.Some abbreviatedType1]" and
+      e = "App (Fun f ts) (Var 0)" and
+      v' = "VPrim (LU32 r)" and
+      \<tau>  = "TPrim (Num U32)" in val.rename_monoexpr_correct(1)
+      [OF _ val_proc_env_matches_\<xi>m_\<Xi> value_sem_rename_mono_prog_rename_\<Xi>_\<xi>m_\<xi>p]; clarsimp?)
+     apply (clarsimp simp: abbreviatedType1_def)
+     apply (clarsimp simp: val.matches_Cons[where xs = "[]" and ys = "[]", simplified])
+     apply (clarsimp simp: val.matches_def)
+     apply (rule val.v_t_record; simp?)
+     apply (rule val.v_t_r_cons1; clarsimp?)
+      apply (rule val.v_t_prim'; clarsimp)
+     apply (rule val.v_t_r_cons1; clarsimp?)
+      apply (rule val.v_t_prim'; clarsimp)
+     apply (rule val.v_t_r_cons1; clarsimp?)
+      apply (rule val.v_t_unit)
+     apply (rule val.v_t_r_empty)
+    apply (case_tac va; clarsimp)
+   apply (subst val_wa_foldnb_bod_0p.simps; clarsimp)
+  apply (clarsimp simp: not_le)
+  apply (frule_tac x = to in spec)
+  apply (erule impE, simp)
+  apply (erule exE)
+  apply (drule val_wa_foldnb_bod_0_back_step; simp?)
+  apply clarsimp
+  apply (subgoal_tac "\<exists>y. r' = VPrim (LU32 y)", clarsimp)
+   apply (erule_tac x = y in meta_allE)
+   apply clarsimp
+   apply (drule_tac \<gamma> = "[VRecord [VPrim (LU32 v), VPrim (LU32 y), VUnit]]" and
+      \<Gamma> = "[option.Some abbreviatedType1]" and
+      e = "App (Fun f ts) (Var 0)" and
+      v' = "VPrim (LU32 r)" and
+      \<tau>  = "TPrim (Num U32)" in val.rename_monoexpr_correct(1)
+      [OF _ val_proc_env_matches_\<xi>m_\<Xi> value_sem_rename_mono_prog_rename_\<Xi>_\<xi>m_\<xi>p]; clarsimp?)
+    apply (clarsimp simp: abbreviatedType1_def)
+    apply (clarsimp simp: val.matches_Cons[where xs = "[]" and ys = "[]", simplified])
+    apply (clarsimp simp: val.matches_def)
+    apply (rule val.v_t_record; simp?)
+    apply (rule val.v_t_r_cons1; clarsimp?)
+     apply (rule val.v_t_prim'; clarsimp)
+    apply (rule val.v_t_r_cons1; clarsimp?)
+     apply (rule val.v_t_prim'; clarsimp)
+    apply (rule val.v_t_r_cons1; clarsimp?)
+     apply (rule val.v_t_unit)
+    apply (rule val.v_t_r_empty)
+   apply (case_tac va; clarsimp)
+   apply (drule_tac v = v and r' = "VPrim (LU32 r)" in val_wa_foldnb_bod_0p_step; simp)
+  apply (insert val_proc_env_matches_\<xi>m_\<Xi>)
+  apply (drule val_wa_foldnb_bod_0_preservation; simp?)
+    apply (rule val.v_t_prim[where l = "LU32 _", simplified])
+   apply clarsimp
+   apply (erule v_t_prim_tE)
+   apply (drule lit_type_ex_32[OF sym])
+  apply clarsimp
+  apply (clarsimp simp: abbreviatedType1_def)
+   apply (clarsimp simp: val.matches_Cons[where xs = "[]" and ys = "[]", simplified])
+   apply (clarsimp simp: val.matches_def)
+   apply (rule val.v_t_record; simp?)
+   apply (rule val.v_t_r_cons1; clarsimp?)
+    apply (rule val.v_t_prim'; clarsimp)
+   apply (rule val.v_t_r_cons1; clarsimp?)
+    apply (rule val.v_t_prim'; clarsimp)
+   apply (rule val.v_t_r_cons1; clarsimp?)
+    apply (rule val.v_t_unit)
+   apply (rule val.v_t_r_empty)
+  apply (erule v_t_prim_tE)
+  apply (drule lit_type_ex_32[OF sym])
+  apply clarsimp
+  done
+
+lemma val_wa_foldnb_0_mono_helper2:
+  "\<lbrakk>val.proc_env_matches \<xi>m1 \<Xi>; proc_ctx_wellformed \<Xi>; \<forall>i<length xs. \<exists>v. xs ! i = VPrim (LU32 v);
+    \<Xi>, [], [option.Some Generated_TypeProof.abbreviatedType1] \<turnstile> App (AFun (rename (f, ts)) []) 
+      (Var 0) : TPrim (Num U32);
+    val_wa_foldnb_bod_0 xs frm to (AFun (rename (f, ts)) [])
+         (VPrim (LU32 acc)) VUnit (VPrim (LU32 r))\<rbrakk>
+       \<Longrightarrow> val_wa_foldnb_bod_0p xs frm to (AFun f ts) (VPrim (LU32 acc)) VUnit (VPrim (LU32 r))"
+  apply (induct to arbitrary: r)
+   apply (erule val_wa_foldnb_bod_0.elims; clarsimp)
+   apply (subst val_wa_foldnb_bod_0p.simps; clarsimp)
+  apply clarsimp
+  apply (case_tac "length xs < Suc to")
+   apply (erule_tac x = r in meta_allE)
+   apply (drule val_wa_foldnb_bod_0_back_step'; simp)
+   apply (drule val_wa_foldnb_bod_0p_to_geq_lenD)
+    apply linarith
+   apply (rule val_wa_foldnb_bod_0p_to_geq_len; simp)
+  apply (clarsimp simp: not_less)
+  apply (case_tac "frm \<ge> to")
+   apply (erule val_wa_foldnb_bod_0.elims; clarsimp split: if_splits)
+    apply (erule val_wa_foldnb_bod_0.elims; clarsimp)
+    apply (subst val_wa_foldnb_bod_0p.simps; clarsimp)
+    apply (subst val_wa_foldnb_bod_0p.simps; clarsimp)
+    apply (drule_tac \<gamma> = "[VRecord [VPrim (LU32 v), VPrim (LU32 acc), VUnit]]" and
+      \<Gamma> = "[option.Some abbreviatedType1]" and
+      e = "App (AFun f ts) (Var 0)" and
+      v' = "VPrim (LU32 r)" and
+      \<tau>  = "TPrim (Num U32)" in val.rename_monoexpr_correct(1)
+      [OF _ val_proc_env_matches_\<xi>m_\<Xi> value_sem_rename_mono_prog_rename_\<Xi>_\<xi>m_\<xi>p]; clarsimp?)
+     apply (clarsimp simp: abbreviatedType1_def)
+     apply (clarsimp simp: val.matches_Cons[where xs = "[]" and ys = "[]", simplified])
+     apply (clarsimp simp: val.matches_def)
+     apply (rule val.v_t_record; simp?)
+     apply (rule val.v_t_r_cons1; clarsimp?)
+      apply (rule val.v_t_prim'; clarsimp)
+     apply (rule val.v_t_r_cons1; clarsimp?)
+      apply (rule val.v_t_prim'; clarsimp)
+     apply (rule val.v_t_r_cons1; clarsimp?)
+      apply (rule val.v_t_unit)
+     apply (rule val.v_t_r_empty)
+    apply (case_tac va; clarsimp)
+   apply (subst val_wa_foldnb_bod_0p.simps; clarsimp)
+  apply (clarsimp simp: not_le)
+  apply (frule_tac x = to in spec)
+  apply (erule impE, simp)
+  apply (erule exE)
+  apply (drule val_wa_foldnb_bod_0_back_step; simp?)
+  apply clarsimp
+  apply (subgoal_tac "\<exists>y. r' = VPrim (LU32 y)", clarsimp)
+   apply (erule_tac x = y in meta_allE)
+   apply clarsimp
+   apply (drule_tac \<gamma> = "[VRecord [VPrim (LU32 v), VPrim (LU32 y), VUnit]]" and
+      \<Gamma> = "[option.Some abbreviatedType1]" and
+      e = "App (AFun f ts) (Var 0)" and
+      v' = "VPrim (LU32 r)" and
+      \<tau>  = "TPrim (Num U32)" in val.rename_monoexpr_correct(1)
+      [OF _ val_proc_env_matches_\<xi>m_\<Xi> value_sem_rename_mono_prog_rename_\<Xi>_\<xi>m_\<xi>p]; clarsimp?)
+    apply (clarsimp simp: abbreviatedType1_def)
+    apply (clarsimp simp: val.matches_Cons[where xs = "[]" and ys = "[]", simplified])
+    apply (clarsimp simp: val.matches_def)
+    apply (rule val.v_t_record; simp?)
+    apply (rule val.v_t_r_cons1; clarsimp?)
+     apply (rule val.v_t_prim'; clarsimp)
+    apply (rule val.v_t_r_cons1; clarsimp?)
+     apply (rule val.v_t_prim'; clarsimp)
+    apply (rule val.v_t_r_cons1; clarsimp?)
+     apply (rule val.v_t_unit)
+    apply (rule val.v_t_r_empty)
+   apply (case_tac va; clarsimp)
+   apply (drule_tac v = v and r' = "VPrim (LU32 r)" in val_wa_foldnb_bod_0p_step; simp)
+  apply (insert val_proc_env_matches_\<xi>m_\<Xi>)
+  apply (drule val_wa_foldnb_bod_0_preservation; simp?)
+    apply (rule val.v_t_prim[where l = "LU32 _", simplified])
+   apply clarsimp
+   apply (erule v_t_prim_tE)
+   apply (drule lit_type_ex_32[OF sym])
+  apply clarsimp
+  apply (clarsimp simp: abbreviatedType1_def)
+   apply (clarsimp simp: val.matches_Cons[where xs = "[]" and ys = "[]", simplified])
+   apply (clarsimp simp: val.matches_def)
+   apply (rule val.v_t_record; simp?)
+   apply (rule val.v_t_r_cons1; clarsimp?)
+    apply (rule val.v_t_prim'; clarsimp)
+   apply (rule val.v_t_r_cons1; clarsimp?)
+    apply (rule val.v_t_prim'; clarsimp)
+   apply (rule val.v_t_r_cons1; clarsimp?)
+    apply (rule val.v_t_unit)
+   apply (rule val.v_t_r_empty)
+  apply (erule v_t_prim_tE)
+  apply (drule lit_type_ex_32[OF sym])
+  apply clarsimp
+  done
+
+lemma value_sem_rename_mono_prog_rename_\<Xi>_\<xi>m1_\<xi>p1: 
+  "value_sem.rename_mono_prog abs_typing_v rename \<Xi> \<xi>m1 \<xi>p1"
+  apply (clarsimp simp: val.rename_mono_prog_def)
+  apply (rule conjI; clarsimp)
+   apply (rule_tac x = v' in exI)
+   apply (subst (asm) rename_def)
+   apply (subst (asm) assoc_lookup.simps)+
+   apply (clarsimp split: if_split_asm simp: val_wa_length_0_def)
+   apply (case_tac v; clarsimp)
+  apply (rule conjI; clarsimp)
+   apply (rule_tac x = v' in exI)
+   apply (subst (asm) rename_def)
+   apply (subst (asm) assoc_lookup.simps)+
+   apply (clarsimp split: if_split_asm simp: val_wa_get_0_def)
+   apply (case_tac v; clarsimp)
+   apply (case_tac z; clarsimp)
+   apply (case_tac za; clarsimp)
+  apply (rule conjI; clarsimp)
+   apply (rule_tac x = v' in exI)
+   apply (subst (asm) rename_def)
+   apply (subst (asm) assoc_lookup.simps)+
+   apply (clarsimp split: if_split_asm simp: val_wa_put2_0_def)
+   apply (case_tac v; clarsimp)
+   apply (case_tac z; clarsimp)
+   apply (case_tac za; clarsimp)
+   apply (case_tac zb; clarsimp)
+  apply (subst (asm) rename_def)
+  apply (subst (asm) assoc_lookup.simps)+
+  apply (clarsimp split: if_split_asm simp: val_wa_foldnb_0_def val_wa_foldnb_0p_def)
+  apply (case_tac v; clarsimp)
+  apply (case_tac x4; clarsimp)
+  apply (case_tac a; clarsimp)
+  apply (case_tac list; clarsimp)
+  apply (case_tac a; clarsimp)
+  apply (case_tac lista; clarsimp)
+  apply (case_tac a; clarsimp)
+  apply (case_tac list; clarsimp)
+  apply (case_tac lista; clarsimp)
+  apply (case_tac aa; clarsimp)
+  apply (case_tac list; clarsimp)
+  apply (case_tac aa; clarsimp)
+  apply (rule_tac x = "VPrim (LU32 r)" in exI)
+  apply clarsimp
+  apply (case_tac a; clarsimp)
+   apply (clarsimp simp: val_wa_foldnb_0_mono_helper1)
+  apply (clarsimp simp: val_wa_foldnb_0_mono_helper2)
+  done
+
+
+lemma 
+  "\<lbrakk>val_wa_foldnb_bod_0 xs frm (Suc to) f acc obsv r; frm < Suc to\<rbrakk>
+    \<Longrightarrow> \<exists>acc'. val_wa_foldnb_bod_0 xs to (Suc to) f acc' obsv r"
+  apply (induct rule: val_wa_foldnb_bod_0.induct[where ?a0.0 = xs and
+                                                       ?a1.0 = frm and
+                                                       ?a2.0 = to and
+                                                       ?a3.0 = f and
+                                                       ?a4.0 = acc and
+                                                       ?a5.0 = obsv and
+                                                       ?a6.0 = r]; clarsimp)
+  apply (case_tac "frm < length xs")
+   apply (case_tac "frm < to")
+    apply (erule val_wa_foldnb_bod_0.elims; clarsimp)
+   apply clarsimp
+   apply (rule_tac x = acc in exI)
+   apply (erule val_wa_foldnb_bod_0.elims; clarsimp)+
+   apply (subst val_wa_foldnb_bod_0.simps; clarsimp)+
+   apply (rule_tac x = v in exI)
+   apply clarsimp
+   apply (subgoal_tac "frma = to")
+    apply clarsimp
+   apply linarith
+  apply (rule_tac x = res in exI)
+  apply (subst val_wa_foldnb_bod_0.simps; clarsimp)
+  done
+lemma 
+  "\<lbrakk>val_wa_foldnb_bod_0 xs frm to f (VPrim (LU32 acc)) VUnit r; 
+    \<forall>i<length xs. \<exists>v. xs ! i = VPrim (LU32 v);
+    \<Xi>, [], [option.Some abbreviatedType1] \<turnstile> App f (Var 0) : TPrim (Num U32)\<rbrakk>
+    \<Longrightarrow> \<exists>x. r = VPrim (LU32 x)"
+  apply (induct to arbitrary: r)
+   apply (erule val_wa_foldnb_bod_0.elims; clarsimp)
+  apply (case_tac "length xs < Suc to")
+   apply (drule val_wa_foldnb_bod_0_back_step'; simp)
+  apply (case_tac "to \<le> frm")
+   apply (erule val_wa_foldnb_bod_0.elims; clarsimp split: if_splits)
+   apply (erule val_wa_foldnb_bod_0.elims; clarsimp)
+   apply (insert proc_ctx_wellformed_\<Xi> val_proc_env_matches_\<xi>m_\<Xi>)
+   apply (drule val.preservation(1)[of "[]" "[]" _ _ _  \<xi>m, simplified]; simp?)
+    apply (clarsimp simp: abbreviatedType1_def)
+    apply (clarsimp simp: val.matches_Cons[where xs = "[]" and ys = "[]", simplified])
+    apply (clarsimp simp: val.matches_def)
+    apply (rule val.v_t_record; simp?)
+    apply (rule val.v_t_r_cons1; clarsimp?)
+     apply (rule val.v_t_prim'; clarsimp)
+    apply (rule val.v_t_r_cons1; clarsimp?)
+     apply (rule val.v_t_prim'; clarsimp)
+    apply (rule val.v_t_r_cons1; clarsimp?)
+     apply (rule val.v_t_unit)
+    apply (rule val.v_t_r_empty)
+   apply (erule v_t_prim_tE; clarsimp simp: lit_type_ex_32)
+  apply (clarsimp simp: not_less not_le)
+  apply (erule_tac x = to in allE; clarsimp)
+  apply (drule val_wa_foldnb_bod_0_back_step; simp?)
+  apply clarsimp
+  apply (drule_tac x = r' in meta_spec)
+  apply clarsimp
+  apply (insert proc_ctx_wellformed_\<Xi> val_proc_env_matches_\<xi>m_\<Xi>)
+  apply (drule val.preservation(1)[of "[]" "[]" _ _ _  \<xi>m, simplified]; simp?)
+   apply (clarsimp simp: abbreviatedType1_def)
+   apply (clarsimp simp: val.matches_Cons[where xs = "[]" and ys = "[]", simplified])
+   apply (clarsimp simp: val.matches_def)
+   apply (rule val.v_t_record; simp?)
+   apply (rule val.v_t_r_cons1; clarsimp?)
+    apply (rule val.v_t_prim'; clarsimp)
+   apply (rule val.v_t_r_cons1; clarsimp?)
+    apply (rule val.v_t_prim'; clarsimp)
+   apply (rule val.v_t_r_cons1; clarsimp?)
+    apply (rule val.v_t_unit)
+   apply (rule val.v_t_r_empty)
+  apply (erule v_t_prim_tE; clarsimp simp: lit_type_ex_32)
+  done
+
+(*
+
+lemma wordarray_fold_no_break_upd_val:
+  "\<And>K a b \<sigma> \<sigma>' \<tau>s aa a' v v' r w.
+   \<lbrakk>list_all2 (kinding []) \<tau>s K; wordarray_fold_no_break_0_type = (K, a, b); 
+    upd_val_rel \<Xi> \<sigma> aa a' (instantiate \<tau>s a) r w; upd_wa_foldnb_0 (\<sigma>, aa) (\<sigma>', v)\<rbrakk>
+    \<Longrightarrow> (val_wa_foldnb_0 a' v' \<longrightarrow> (\<exists>r' w'. upd_val_rel \<Xi> \<sigma>' v v' (instantiate \<tau>s b) r' w' \<and> r' \<subseteq> r \<and>
+          frame \<sigma> w \<sigma>' w')) \<and> Ex (val_wa_foldnb_0 a')"
+  apply (clarsimp simp: wordarray_fold_no_break_0_type_def upd_wa_foldnb_0_def)
+  apply (case_tac fs; clarsimp)
+  apply (case_tac list; clarsimp)
+  apply (case_tac lista; clarsimp)
+  apply (case_tac list; clarsimp)
+  apply (case_tac lista; clarsimp)
+  apply (case_tac list; clarsimp)
+  apply (rule conjI)
+   apply (case_tac x; clarsimp)
+    apply (case_tac y; clarsimp)
+    apply (rule_tac x = "{}" in exI)+
+    apply clarsimp
+    apply (rule conjI)
+     apply (clarsimp simp: val_wa_foldnb_0_def)
+     apply (case_tac fs; clarsimp)
+     apply (case_tac list; clarsimp)
+     apply (case_tac lista; clarsimp)
+     apply (case_tac list; clarsimp)
+     apply (case_tac lista; clarsimp)
+     apply (case_tac list; clarsimp)
+     apply (case_tac a; clarsimp)
+      apply (erule u_v_recE; clarsimp)
+      apply (erule u_v_r_consE; clarsimp)
+      apply (erule u_v_p_absE; clarsimp)
+      apply (erule u_v_r_consE; simp)
+      apply (erule conjE)+
+      apply (subst (asm) type_repr.simps[symmetric])+
+      apply clarsimp
+      apply (erule u_v_primE)  
+      apply (subst (asm) lit_type.simps)
+      apply clarsimp
+      apply (erule u_v_r_consE; simp)
+      apply (erule conjE)+
+      apply (subst (asm) type_repr.simps[symmetric])+
+      apply clarsimp
+      apply (erule u_v_primE)  
+      apply (subst (asm) lit_type.simps)
+      apply clarsimp
+      apply (erule u_v_r_consE; simp)
+      apply (erule conjE)+
+      apply (subst (asm) type_repr.simps[symmetric])+
+      apply clarsimp
+      apply (erule u_v_functionE; clarsimp)
+      apply (erule u_v_r_consE; simp)
+      apply (erule conjE)+
+      apply (subst (asm) type_repr.simps[symmetric])+
+      apply clarsimp
+      apply (erule u_v_primE)  
+      apply (subst (asm) lit_type.simps)
+      apply clarsimp
+      apply (erule u_v_r_consE; simp)
+      apply (erule conjE)+
+      apply (subst (asm) type_repr.simps[symmetric])+
+      apply clarsimp
+      apply (erule u_v_r_emptyE; clarsimp)
+      apply (subst upd_val_rel.simps; clarsimp)
+      apply (subst (asm) upd_val_rel.simps; clarsimp)
+      apply (erule disjE)
+       apply clarsimp
+      apply (erule disjE; clarsimp)
+      apply (thin_tac "_, _, _ \<turnstile> _ : _")
+      apply (thin_tac "list_all2 _ _ _")
+      apply (thin_tac "type_wellformed _ _")
+      apply (thin_tac "_ \<turnstile> _ \<sqsubseteq> _")
+      apply (clarsimp simp: abs_upd_val'_def)
+      apply (induct arbitrary: \<sigma>' p frm x61 x62 acc ra xs rb len arr
+                    rule: word_induct2[where n = to])
+  thm word_induct
+  find_theorems name:"word" name:"induct"
+  
+
+(*
+      apply (erule u_v_r_consE; simp)
+      apply (erule conjE)+
+      apply (subst (asm) type_repr.simps[symmetric])+
+      apply clarsimp
+      apply (erule u_v_r_consE; simp)
+      apply (erule conjE)+
+      apply (subst (asm) type_repr.simps[symmetric])+
+      apply clarsimp
+      apply (erule u_v_r_consE; simp)
+      apply (erule conjE)+
+      apply (subst (asm) type_repr.simps[symmetric])+
+      apply clarsimp
+      apply (erule u_v_r_consE; simp)
+      apply (erule conjE)+
+      apply (subst (asm) type_repr.simps[symmetric])+
+      apply clarsimp
+*)
+  oops
+  
+
+lemma 
+  "\<lbrakk>val_wa_foldnb_bod_0 xs frm to f acc obsv r; val_wa_foldnb_bod_0 xs frm to f acc obsv r'\<rbrakk>
+    \<Longrightarrow> r = r'"
+  apply (induct to)
+ 
+(*
+  apply (induct arbitrary: r'
+                rule: val_wa_foldnb_bod_0.induct; clarsimp)
+  apply (erule val_wa_foldnb_bod_0.elims)
+  apply (clarsimp split: if_splits)
+   apply (drule_tac x = acc' in meta_spec)
+   apply (drule_tac x = r' in meta_spec)
+   apply (drule meta_mp)
+    apply simp
+   apply (erule val_wa_foldnb_bod_0.elims; clarsimp)
+   apply (erule meta_impE)
+    apply (erule v_sem_appE)
+     apply (erule v_sem_varE; clarsimp simp: val_wa_put2_0_def val_wa_get_0_def val_wa_length_0_def)
+    apply (erule v_sem_appE)
+     apply (erule v_sem_varE)+
+     apply (clarsimp simp: val_wa_put2_0_def val_wa_get_0_def val_wa_length_0_def)
+    apply (erule v_sem_varE)+
+    apply clarsimp
+  find_theorems "?xs ! ?i" "length ?xs \<le> ?i"
+  
+  find_theorems "( _ , _ \<turnstile> _ \<Down> _) \<and>  (_ , _ \<turnstile> _ \<Down> _)"
+  *)
+
+  oops
+lemma 
+  "\<lbrakk>upd_wa_foldnb_bod_0 \<sigma> p frm to f (UPrim (LU32 acc), RPrim (Num U32)) (UUnit, RUnit) (\<sigma>', UPrim (LU32 ra));
+    abs_upd_val' (WAU32 len arr) (VWA xs) ''WordArray'' [TPrim (Num U32)] (Boxed ReadOnly undefined) r w \<sigma>\<rbrakk>
+    \<Longrightarrow> val_wa_foldnb_bod_0 xs (unat frm) (unat to) f (VPrim (LU32 acc)) VUnit (VPrim (LU32 ra))"
+  apply (induct arbitrary: \<sigma>' ra rule: word_induct[where m = "to"])
+   apply (erule upd_wa_foldnb_bod_0.elims; clarsimp)
+   apply (subst val_wa_foldnb_bod_0.simps; clarsimp)
+  apply clarsimp
+  apply (case_tac "1 + n \<le> 0")
+   apply (erule upd_wa_foldnb_bod_0.elims; clarsimp)
+   apply (subst val_wa_foldnb_bod_0.simps; clarsimp)
+  apply (simp add: word_gt_0)
+  apply (drule unatSuc; clarsimp)
+(*
+  apply (drule upd_wa_foldnb_bod_0_back_step; clarsimp)
+   apply (simp add: word_gt_0)
+
+  thm val_wa_foldnb_bod_0_step val_executes_from_upd_executes(1) correspondence(1) specialisation(1)
+  find_theorems "?\<Xi>, _, ?\<Gamma> \<turnstile> specialise _ _ : ?\<tau>"
+  thm typing_appE
+
+*)
+  thm val_executes_from_upd_executes(1) correspondence(1) specialisation(1) mono_correspondence(1)
+  oops
+  thm v_sem_primE
+lemma "\<lbrakk>\<xi>m , \<gamma> \<turnstile> e \<Down> v; \<xi>m , \<gamma> \<turnstile> e \<Down> v'\<rbrakk> \<Longrightarrow> v = v'"
+  apply (induct e)
+                      apply (erule v_sem_varE; clarsimp)+
+                      apply (erule v_sem_afunE; clarsimp)+
+                     apply (erule v_sem_funE; clarsimp)+
+                    apply (erule v_sem_primE; clarsimp)+
+  
+                    defer
+                    defer
+                    apply (erule v_sem_conE; clarsimp)+
+                    defer
+                    apply (erule v_sem_structE; clarsimp)+
+  defer
+
+  oops
+*)
 end (* of context *)
 
 end
